aspec: refactor det_ext to remove scheduler state
The scheduler is now fully part of the extensible abstract
specification, because we are increasingly finding properties that are
not able to be reasonably specified without it. This means that there is
now no non-deterministic scheduler specification and that the only slots
for non-determinism are now CDT and preemption operations.

This came up due to some properties currently being proved not being
true for all execution paths of the previous non-deterministic
specification. Options that were considered were:
1 - move the minimal state (the current domain and tcb's domain)
required for the properties currently being considered to the extensible
abstract specification.
2 - move all of the scheduler state to the extensible abstract
specification, the same as what has been done on the rt branch.
3 - move all state and remove the non-deterministic specification
completely.
4 - add ghost state to sidestep the specific problem that we are
currently encountering (it is unclear whether this would actually work).

Option 2 was chosen because it is the least blocking (although may be
more annoying than some of the others), will result in the smallest diff
to the rt branch, and we don't think it will be significantly more work
than option 1. If we want to reason about threads in the
future (e.g. liveness), we will require that this information about the
scheduler state is accessible.

We are really not sure about whether moving specifically the scheduler
action is the right decision, but we are moving it across because the
correctness of the ready queues depends on it and any alternatives that
we have thought of would be a lot of work that we do not want to do at
this time.

Signed-off-by: Corey Lewis <corey.lewis@proofcraft.systems>

spec/abstract/Deterministic_A.thy
@@ -25,7 +25,7 @@ The basic technique, and its motivation, are described in~\cite{Matichuk_Murray_
 
 Here, we define two such instantiations. The first yields a
 largely-deterministic specification by instantiating @{typ "'a"} with
-a record that includes concrete scheduler state and
+a record that includes
 information about sibling ordering in the capability derivation tree (CDT).
 We call the resulting
 specification the \emph{deterministic abstract specification} and it is
@@ -33,8 +33,8 @@ defined below in \autoref{s:det-spec}.
 
 The second instantiation uses the type @{typ unit} for @{typ 'a}, yielding
 a specification that is far more nondeterministic. In particular, the
-scheduling behaviour and the order in which capabilities are deleted during
-a \emph{revoke} system call both become completely nondeterministic.
+order in which capabilities are deleted during
+a \emph{revoke} system call becomes completely nondeterministic.
 We call this second instantiation the
 \emph{nondeterministic abstract specification} and it is defined below in
 \autoref{s:nondet-spec}.
@@ -44,52 +44,54 @@ text \<open>Translate a state of type @{typ "'a state"} to one of type @{typ "'b
   via a function @{term t} from @{typ "'a"} to @{typ "'b"}.
 \<close>
 definition trans_state :: "('a \<Rightarrow> 'b) \<Rightarrow> 'a state \<Rightarrow> 'b state" where
-"trans_state t s = \<lparr>kheap = kheap s, cdt = cdt s, is_original_cap = is_original_cap s,
-                     cur_thread = cur_thread s, idle_thread = idle_thread s,
-                     machine_state = machine_state s,
-                     interrupt_irq_node = interrupt_irq_node s,
-                     interrupt_states = interrupt_states s, arch_state = arch_state s,
-                     exst = t(exst s)\<rparr>"
+  "trans_state t s = abstract_state.extend (abstract_state.truncate s) (state.fields (t (exst s)))"
 
 (*<*)
-lemma trans_state[simp]: "kheap (trans_state t s) = kheap s"
-                            "cdt (trans_state t s) = cdt s"
-                            "is_original_cap (trans_state t s) = is_original_cap s"
-                            "cur_thread (trans_state t s) = cur_thread s"
-                            "idle_thread (trans_state t s) = idle_thread s"
-                            "machine_state (trans_state t s) = machine_state s"
-                            "interrupt_irq_node (trans_state t s) = interrupt_irq_node s"
-                           "interrupt_states (trans_state t s) = interrupt_states s"
-                            "arch_state (trans_state t s) = arch_state s"
-                            "exst (trans_state t s) = (t (exst s))"
-                            "exst (trans_state (\<lambda>_. e) s) = e"
-  apply (simp add: trans_state_def)+
-  done
+lemma trans_state[simp]:
+  "kheap (trans_state t s) = kheap s"
+  "cdt (trans_state t s) = cdt s"
+  "is_original_cap (trans_state t s) = is_original_cap s"
+  "cur_thread (trans_state t s) = cur_thread s"
+  "idle_thread (trans_state t s) = idle_thread s"
+  "machine_state (trans_state t s) = machine_state s"
+  "interrupt_irq_node (trans_state t s) = interrupt_irq_node s"
+  "interrupt_states (trans_state t s) = interrupt_states s"
+  "arch_state (trans_state t s) = arch_state s"
+  "scheduler_action (trans_state t s) = scheduler_action s"
+  "domain_list (trans_state t s) = domain_list s"
+  "domain_index (trans_state t s) = domain_index s"
+  "cur_domain (trans_state t s) = cur_domain s"
+  "domain_time (trans_state t s) = domain_time s"
+  "ready_queues (trans_state t s) = ready_queues s"
+  "exst (trans_state t s) = (t (exst s))"
+  "exst (trans_state (\<lambda>_. e) s) = e"
+  by (simp add: trans_state_def abstract_state.defs state.defs)+
 
 lemma trans_state_update[simp]:
- "trans_state t (kheap_update f s) = kheap_update f (trans_state t s)"
- "trans_state t (cdt_update g s) = cdt_update g (trans_state t s)"
- "trans_state t (is_original_cap_update h s) = is_original_cap_update h (trans_state t s)"
- "trans_state t (cur_thread_update i s) = cur_thread_update i (trans_state t s)"
- "trans_state t (idle_thread_update j s) = idle_thread_update j (trans_state t s)"
- "trans_state t (machine_state_update k s) = machine_state_update k (trans_state t s)"
- "trans_state t (interrupt_irq_node_update l s) = interrupt_irq_node_update l (trans_state t s)"
- "trans_state t (arch_state_update m s) = arch_state_update m (trans_state t s)"
- "trans_state t (interrupt_states_update p s) = interrupt_states_update p (trans_state t s)"
-  apply (simp add: trans_state_def)+
-  done
+  "trans_state t (kheap_update f s) = kheap_update f (trans_state t s)"
+  "trans_state t (cdt_update g s) = cdt_update g (trans_state t s)"
+  "trans_state t (is_original_cap_update h s) = is_original_cap_update h (trans_state t s)"
+  "trans_state t (cur_thread_update i s) = cur_thread_update i (trans_state t s)"
+  "trans_state t (idle_thread_update j s) = idle_thread_update j (trans_state t s)"
+  "trans_state t (machine_state_update k s) = machine_state_update k (trans_state t s)"
+  "trans_state t (interrupt_irq_node_update l s) = interrupt_irq_node_update l (trans_state t s)"
+  "trans_state t (arch_state_update m s) = arch_state_update m (trans_state t s)"
+  "trans_state t (scheduler_action_update b s) = scheduler_action_update b (trans_state t s)"
+  "trans_state t (domain_list_update c s) = domain_list_update c (trans_state t s)"
+  "trans_state t (domain_index_update d s) = domain_index_update d (trans_state t s)"
+  "trans_state t (cur_domain_update e s) = cur_domain_update e (trans_state t s)"
+  "trans_state t (domain_time_update f2 s) = domain_time_update f2 (trans_state t s)"
+  "trans_state t (ready_queues_update g2 s) = ready_queues_update g2 (trans_state t s)"
+  by (simp add: trans_state_def abstract_state.defs)+
 
 
 lemma trans_state_update':
   "trans_state f = exst_update f"
-  apply (rule ext)
-  apply simp
-  done
+  by (rule ext) simp
 
 lemma trans_state_update''[simp]:
   "trans_state t' (trans_state t s) = trans_state (\<lambda>e. t' (t e)) s"
-  apply simp
-  done
+  by simp
 (*>*)
 
 text \<open>Truncate an extended state of type @{typ "'a state"}
@@ -100,33 +102,8 @@ abbreviation "truncate_state \<equiv> trans_state (\<lambda>_. ())"
 section "Deterministic Abstract Specification"
 
 text \<open>\label{s:det-spec}
-  The deterministic abstract specification tracks the state of the scheduler
-and ordering information about sibling nodes in the CDT.\<close>
-
-text \<open>The current scheduler action,
-  which is part of the scheduling state.\<close>
-datatype scheduler_action =
-    resume_cur_thread
-  | switch_thread (sch_act_target : obj_ref)
-  | choose_new_thread
-
-type_synonym domain = word8
-
-record etcb =
- tcb_priority :: "priority"
- tcb_time_slice :: "nat"
- tcb_domain :: "domain"
-
-definition default_priority :: "priority" where
-  "default_priority \<equiv> minBound"
-
-definition default_domain :: "domain" where
-  "default_domain \<equiv> minBound"
-
-definition default_etcb :: "etcb" where
-  "default_etcb \<equiv> \<lparr>tcb_priority = default_priority, tcb_time_slice = timeSlice, tcb_domain = default_domain\<rparr>"
-
-type_synonym ready_queue = "obj_ref list"
+  The deterministic abstract specification tracks
+  ordering information about sibling nodes in the CDT.\<close>
 
 text \<open>
   For each entry in the CDT, we record an ordered list of its children.
@@ -141,13 +118,6 @@ text \<open>
 \<close>
 record det_ext =
    work_units_completed_internal :: "machine_word"
-   scheduler_action_internal :: scheduler_action
-   ekheap_internal :: "obj_ref \<Rightarrow> etcb option"
-   domain_list_internal :: "(domain \<times> machine_word) list"
-   domain_index_internal :: nat
-   cur_domain_internal :: domain
-   domain_time_internal :: "machine_word"
-   ready_queues_internal :: "domain \<Rightarrow> priority \<Rightarrow> ready_queue"
    cdt_list_internal :: cdt_list
 
 text \<open>
@@ -166,48 +136,6 @@ abbreviation
   "work_units_completed_update f (s::det_state) \<equiv>  trans_state (work_units_completed_internal_update f) s"
 
 abbreviation
-  "scheduler_action (s::det_state) \<equiv> scheduler_action_internal (exst s)"
-
-abbreviation
-  "scheduler_action_update f (s::det_state) \<equiv>  trans_state (scheduler_action_internal_update f) s"
-
-abbreviation
-  "ekheap (s::det_state) \<equiv> ekheap_internal (exst s)"
-
-abbreviation
-  "ekheap_update f (s::det_state) \<equiv> trans_state (ekheap_internal_update f) s"
-
-abbreviation
-  "domain_list (s::det_state) \<equiv> domain_list_internal (exst s)"
-
-abbreviation
-  "domain_list_update f (s::det_state) \<equiv> trans_state (domain_list_internal_update f) s"
-
-abbreviation
-  "domain_index (s::det_state) \<equiv> domain_index_internal (exst s)"
-
-abbreviation
-  "domain_index_update f (s::det_state) \<equiv> trans_state (domain_index_internal_update f) s"
-
-abbreviation
-  "cur_domain (s::det_state) \<equiv> cur_domain_internal (exst s)"
-
-abbreviation
-  "cur_domain_update f (s::det_state) \<equiv> trans_state (cur_domain_internal_update f) s"
-
-abbreviation
-  "domain_time (s::det_state) \<equiv> domain_time_internal (exst s)"
-
-abbreviation
-  "domain_time_update f (s::det_state) \<equiv> trans_state (domain_time_internal_update f) s"
-
-abbreviation
-  "ready_queues (s::det_state) \<equiv> ready_queues_internal (exst s)"
-
-abbreviation
-  "ready_queues_update f (s::det_state) \<equiv> trans_state (ready_queues_internal_update f) s"
-
-abbreviation
   "cdt_list (s::det_state) \<equiv> cdt_list_internal (exst s)"
 
 abbreviation
@@ -215,140 +143,85 @@ abbreviation
 
 type_synonym 'a det_ext_monad = "(det_state,'a) nondet_monad"
 
+
+section \<open>Type Class\<close>
+
 text \<open>
-  Basic monadic functions for operating on the extended state of the
-  deterministic abstract specification.
+  A type class for all instantiations of the abstract specification. In
+  practice, this is restricted to basically allow only two sensible
+  implementations at present: the deterministic abstract specification and
+  the nondeterministic one.
 \<close>
-definition
-  get_etcb :: "obj_ref \<Rightarrow> det_state \<Rightarrow> etcb option"
-where
-  "get_etcb tcb_ref es \<equiv> ekheap es tcb_ref"
-
-definition
-  ethread_get :: "(etcb \<Rightarrow> 'a) \<Rightarrow> obj_ref \<Rightarrow> 'a det_ext_monad"
-where
-  "ethread_get f tptr \<equiv> do
-     tcb \<leftarrow> gets_the $ get_etcb tptr;
-     return $ f tcb
-   od"
-
-(* For infoflow, we want to avoid certain read actions, such as reading the priority of the
-   current thread when it could be idle. Then we need to make sure we do not rely on the result.
-   undefined is the closest we have to a result that can't be relied on *)
-definition
-  ethread_get_when :: "bool \<Rightarrow> (etcb \<Rightarrow> 'a) \<Rightarrow> obj_ref \<Rightarrow> 'a det_ext_monad"
-where
-  "ethread_get_when b f tptr \<equiv> if b then (ethread_get f tptr) else return undefined"
-
-definition set_eobject :: "obj_ref \<Rightarrow> etcb \<Rightarrow> unit det_ext_monad"
-  where
- "set_eobject ptr obj \<equiv>
-  do es \<leftarrow> get;
-    ekh \<leftarrow> return $ (ekheap es)(ptr \<mapsto> obj);
-    put (es\<lparr>ekheap := ekh\<rparr>)
-  od"
-
-definition
-  ethread_set :: "(etcb \<Rightarrow> etcb) \<Rightarrow> obj_ref \<Rightarrow> unit det_ext_monad"
-where
-  "ethread_set f tptr \<equiv> do
-     tcb \<leftarrow> gets_the $ get_etcb tptr;
-     set_eobject tptr $ f tcb
-   od"
-
-definition
-  set_scheduler_action :: "scheduler_action \<Rightarrow> unit det_ext_monad" where
-  "set_scheduler_action action \<equiv>
-     modify (\<lambda>es. es\<lparr>scheduler_action := action\<rparr>)"
-
-definition
-  thread_set_priority :: "obj_ref \<Rightarrow> priority \<Rightarrow> unit det_ext_monad" where
-  "thread_set_priority tptr prio \<equiv> ethread_set (\<lambda>tcb. tcb\<lparr>tcb_priority := prio\<rparr>) tptr"
-
-definition
-  thread_set_time_slice :: "obj_ref \<Rightarrow> nat \<Rightarrow> unit det_ext_monad" where
-  "thread_set_time_slice tptr time \<equiv> ethread_set (\<lambda>tcb. tcb\<lparr>tcb_time_slice := time\<rparr>) tptr"
-
-definition
-  thread_set_domain :: "obj_ref \<Rightarrow> domain \<Rightarrow> unit det_ext_monad" where
-  "thread_set_domain tptr domain \<equiv> ethread_set (\<lambda>tcb. tcb\<lparr>tcb_domain := domain\<rparr>) tptr"
+class state_ext =
+ fixes unwrap_ext :: "'a state \<Rightarrow> det_ext state"
+ fixes wrap_ext :: "(det_ext \<Rightarrow> det_ext) \<Rightarrow> ('a \<Rightarrow> 'a)"
+ fixes wrap_ext_op :: "unit det_ext_monad \<Rightarrow> ('a state,unit) nondet_monad"
+ fixes wrap_ext_bool :: "bool det_ext_monad \<Rightarrow> ('a state,bool) nondet_monad"
+ fixes select_switch :: "'a \<Rightarrow> bool"
+ fixes ext_init :: "'a"
 
 
-definition
-  get_tcb_queue :: "domain \<Rightarrow> priority \<Rightarrow> ready_queue det_ext_monad" where
-  "get_tcb_queue d prio \<equiv> do
-     queues \<leftarrow> gets ready_queues;
-     return (queues d prio)
-   od"
+section \<open>Type Class Instances\<close>
 
-definition
-  set_tcb_queue :: "domain \<Rightarrow> priority \<Rightarrow> ready_queue \<Rightarrow> unit det_ext_monad" where
-  "set_tcb_queue d prio queue \<equiv>
-     modify (\<lambda>es. es\<lparr> ready_queues :=
-      (\<lambda>d' p. if d' = d \<and> p = prio then queue else ready_queues es d' p)\<rparr>)"
+subsection "Deterministic Abstract Specification"
+
+instantiation  det_ext_ext :: (type) state_ext
+begin
+
+definition "unwrap_ext_det_ext_ext == (\<lambda>x. x) :: det_ext state \<Rightarrow> det_ext state"
+
+definition "wrap_ext_det_ext_ext == (\<lambda>x. x) ::
+  (det_ext \<Rightarrow> det_ext) \<Rightarrow> det_ext \<Rightarrow> det_ext"
+
+definition "wrap_ext_op_det_ext_ext == (\<lambda>x. x) ::
+  (det_ext state \<Rightarrow> ((unit \<times> det_ext state) set) \<times> bool)
+  \<Rightarrow> det_ext state  \<Rightarrow> ((unit \<times> det_ext state) set) \<times> bool"
+
+definition "wrap_ext_bool_det_ext_ext == (\<lambda>x. x) ::
+  (det_ext state \<Rightarrow> ((bool \<times> det_ext state) set) \<times> bool)
+  \<Rightarrow> det_ext state \<Rightarrow> ((bool \<times> det_ext state) set) \<times> bool"
+
+definition "select_switch_det_ext_ext == (\<lambda>_. True)  :: det_ext\<Rightarrow> bool"
+
+definition "ext_init_det_ext_ext \<equiv>
+     \<lparr>work_units_completed_internal = 0,
+      cdt_list_internal = const [] \<rparr> :: det_ext"
+
+instance ..
+
+end
+
+subsection "Nondeterministic Abstract Specification"
+
+text \<open>\label{s:nondet-spec}
+The nondeterministic abstract specification instantiates the extended state
+with the unit type -- i.e. it doesn't have any meaningful extended state.
+\<close>
+
+instantiation unit :: state_ext
+begin
+
+definition "unwrap_ext_unit == (\<lambda>_. undefined) :: unit state \<Rightarrow> det_ext state"
+
+definition "wrap_ext_unit == (\<lambda>f s. ()) :: (det_ext \<Rightarrow> det_ext) \<Rightarrow> unit \<Rightarrow> unit"
 
 
-definition
-  tcb_sched_action :: "(obj_ref \<Rightarrow> obj_ref list \<Rightarrow> obj_ref list) \<Rightarrow> obj_ref  \<Rightarrow> unit det_ext_monad" where
-  "tcb_sched_action action thread \<equiv> do
-     d \<leftarrow> ethread_get tcb_domain thread;
-     prio \<leftarrow> ethread_get tcb_priority thread;
-     queue \<leftarrow> get_tcb_queue d prio;
-     set_tcb_queue d prio (action thread queue)
-   od"
+definition "wrap_ext_op_unit == (\<lambda>m. return ()) ::
+  (det_ext state \<Rightarrow> ((unit \<times> det_ext state) set) \<times> bool) \<Rightarrow> unit state \<Rightarrow> ((unit \<times> unit state) set) \<times> bool"
 
-definition
-  tcb_sched_enqueue :: "obj_ref \<Rightarrow> obj_ref list \<Rightarrow> obj_ref list" where
-  "tcb_sched_enqueue thread queue \<equiv> if (thread \<notin> set queue) then thread # queue else queue"
+definition "wrap_ext_bool_unit == (\<lambda>m. select UNIV) ::
+  (det_ext state \<Rightarrow> ((bool \<times> det_ext state ) set) \<times> bool) \<Rightarrow> unit state \<Rightarrow> ((bool \<times> unit state) set) \<times> bool"
 
-definition
-  tcb_sched_append :: "obj_ref \<Rightarrow> obj_ref list \<Rightarrow> obj_ref list" where
-  "tcb_sched_append thread queue \<equiv> if (thread \<notin> set queue) then queue @ [thread] else queue"
+definition "select_switch_unit == (\<lambda>s. False) :: unit \<Rightarrow> bool"
 
-definition
-  tcb_sched_dequeue :: "obj_ref \<Rightarrow> obj_ref list \<Rightarrow> obj_ref list" where
-  "tcb_sched_dequeue thread queue \<equiv> filter (\<lambda>x. x \<noteq> thread) queue"
+definition "ext_init_unit \<equiv> () :: unit"
+
+instance ..
+
+end
 
 
-definition reschedule_required :: "unit det_ext_monad" where
-  "reschedule_required \<equiv> do
-     action \<leftarrow> gets scheduler_action;
-     case action of switch_thread t \<Rightarrow> tcb_sched_action (tcb_sched_enqueue) t | _ \<Rightarrow> return ();
-     set_scheduler_action choose_new_thread
-   od"
-
-definition
-  possible_switch_to :: "obj_ref \<Rightarrow> unit det_ext_monad" where
-  "possible_switch_to target \<equiv> do
-     cur_dom \<leftarrow> gets cur_domain;
-     target_dom \<leftarrow> ethread_get tcb_domain target;
-     action \<leftarrow> gets scheduler_action;
-
-     if (target_dom \<noteq> cur_dom) then
-       tcb_sched_action tcb_sched_enqueue target
-     else if (action \<noteq> resume_cur_thread) then
-       do
-         reschedule_required;
-         tcb_sched_action tcb_sched_enqueue target
-       od
-     else
-       set_scheduler_action $ switch_thread target
-   od"
-
-definition
-  next_domain :: "unit det_ext_monad" where
-  "next_domain \<equiv>
-    modify (\<lambda>s.
-      let domain_index' = (domain_index s + 1) mod length (domain_list s) in
-      let next_dom = (domain_list s)!domain_index'
-      in s\<lparr> domain_index := domain_index',
-            cur_domain := fst next_dom,
-            domain_time := snd next_dom,
-            work_units_completed := 0\<rparr>)"
-
-definition
-  dec_domain_time :: "unit det_ext_monad" where
-  "dec_domain_time = modify (\<lambda>s. s\<lparr>domain_time := domain_time s - 1\<rparr>)"
+section \<open>Basic Deterministic Monadic Accessors\<close>
 
 definition set_cdt_list :: "cdt_list \<Rightarrow> (det_state, unit) nondet_monad" where
   "set_cdt_list t \<equiv> do
@@ -369,9 +242,9 @@ text \<open>The CDT in the implementation is stored in prefix traversal order.
   The following functions traverse its abstract representation here to
   yield corresponding information.
 \<close>
+(* FIXME: use Lib.hd_opt instead *)
 definition next_child :: "cslot_ptr \<Rightarrow> cdt_list \<Rightarrow> cslot_ptr option" where
-  "next_child slot t \<equiv> case (t slot) of [] \<Rightarrow> None |
-                                        x # xs \<Rightarrow> Some x"
+  "next_child slot t \<equiv> case t slot of [] \<Rightarrow> None | x # xs \<Rightarrow> Some x"
 
 definition next_sib :: "cslot_ptr \<Rightarrow> cdt_list \<Rightarrow> cdt \<Rightarrow> cslot_ptr option" where
   "next_sib slot t m \<equiv> case m slot of None \<Rightarrow> None |
@@ -380,10 +253,10 @@ definition next_sib :: "cslot_ptr \<Rightarrow> cdt_list \<Rightarrow> cdt \<Rig
 
 function (domintros) next_not_child :: "cslot_ptr \<Rightarrow> cdt_list \<Rightarrow> cdt \<Rightarrow> cslot_ptr option" where
   "next_not_child slot t m = (if next_sib slot t m = None
-                             then (case m slot of
-                               None \<Rightarrow> None |
-                               Some p \<Rightarrow> next_not_child p t m)
-                             else next_sib slot t m)"
+                              then case m slot of
+                                      None \<Rightarrow> None
+                                    | Some p \<Rightarrow> next_not_child p t m
+                              else next_sib slot t m)"
   by auto
 
 (* next_slot traverses the cdt, replicating mdb_next in the Haskell spec.
@@ -397,24 +270,8 @@ definition next_slot :: "cslot_ptr \<Rightarrow> cdt_list \<Rightarrow> cdt \<Ri
                         then next_child slot t
                         else next_not_child slot t m"
 
+
 text \<open>\emph{Extended operations} for the deterministic abstract specification.\<close>
-
-definition max_non_empty_queue :: "(priority \<Rightarrow> ready_queue) \<Rightarrow> ready_queue" where
-  "max_non_empty_queue queues \<equiv> queues (Max {prio. queues prio \<noteq> []})"
-
-
-definition default_ext :: "apiobject_type \<Rightarrow> domain \<Rightarrow> etcb option" where
-  "default_ext type cdom \<equiv>
-      case type of TCBObject \<Rightarrow> Some (default_etcb\<lparr>tcb_domain := cdom\<rparr>)
-                         | _ \<Rightarrow> None"
-
-definition retype_region_ext :: "obj_ref list \<Rightarrow> apiobject_type \<Rightarrow> unit det_ext_monad" where
-  "retype_region_ext ptrs type \<equiv>  do
-                                     ekh \<leftarrow> gets ekheap;
-                                     cdom \<leftarrow> gets cur_domain;
-                                     ekh' \<leftarrow> return $ foldr (\<lambda>p ekh. (ekh(p := default_ext type cdom))) ptrs ekh;
-                                     modify (\<lambda>s. s\<lparr>ekheap := ekh'\<rparr>)
-                                  od"
 
 definition cap_swap_ext where
 "cap_swap_ext \<equiv> (\<lambda> slot1 slot2 slot1_op slot2_op.
@@ -442,44 +299,44 @@ definition cap_move_ext where
 "cap_move_ext \<equiv> (\<lambda> src_slot dest_slot src_p dest_p.
  do
 
-    update_cdt_list (\<lambda>list. case (dest_p) of
+    update_cdt_list (\<lambda>list. case dest_p of
       None \<Rightarrow> list |
       Some p \<Rightarrow> list (p := list_remove (list p) dest_slot));
 
-   if (src_slot = dest_slot) then return () else
+   if src_slot = dest_slot then return () else
 
     (do
-    update_cdt_list (\<lambda>list. case (src_p) of
+    update_cdt_list (\<lambda>list. case src_p of
       None \<Rightarrow> list |
       Some p \<Rightarrow> list (p := list_replace (list p) src_slot dest_slot));
 
-    update_cdt_list (\<lambda>list. list (src_slot := [], dest_slot := (list src_slot) @ (list dest_slot)))
+    update_cdt_list (\<lambda>list. list (src_slot := [], dest_slot := list src_slot @ list dest_slot))
     od)
 
   od)"
 
 
 definition cap_insert_ext where
-"cap_insert_ext \<equiv> (\<lambda> src_parent src_slot dest_slot src_p dest_p.
- do
-
- update_cdt_list (\<lambda>list. case (dest_p) of
-      None \<Rightarrow> list |
-      Some p \<Rightarrow> (list (p := list_remove (list p) dest_slot)));
-
-    update_cdt_list (\<lambda>list. case (src_p) of
-      None \<Rightarrow> list (
-        src_slot := if src_parent then [dest_slot] @ (list src_slot) else list src_slot) |
-      Some p \<Rightarrow> list (
-        src_slot := if src_parent then [dest_slot] @ (list src_slot) else list src_slot,
-        p := if (src_parent \<and> p \<noteq> src_slot) then (list p) else if (src_slot \<noteq> dest_slot) then (list_insert_after (list p) src_slot dest_slot) else (dest_slot # (list p))))
- od)"
+  "cap_insert_ext \<equiv> \<lambda>src_parent src_slot dest_slot src_p dest_p. do
+     update_cdt_list (\<lambda>list. case dest_p of
+       None \<Rightarrow> list
+     | Some p \<Rightarrow> list (p := list_remove (list p) dest_slot));
+     update_cdt_list (\<lambda>list. case src_p of
+       None \<Rightarrow> list (src_slot := if src_parent then [dest_slot] @ list src_slot else list src_slot)
+     | Some p \<Rightarrow> list (src_slot := if src_parent then [dest_slot] @ list src_slot else list src_slot,
+                       p := if src_parent \<and> p \<noteq> src_slot
+                            then list p
+                            else if src_slot \<noteq> dest_slot
+                                 then list_insert_after (list p) src_slot dest_slot
+                                 else dest_slot # list p))
+   od"
 
 definition empty_slot_ext where
-"empty_slot_ext \<equiv> (\<lambda> slot slot_p.
-
+"empty_slot_ext \<equiv> \<lambda> slot slot_p.
     update_cdt_list (\<lambda>list. case slot_p of None \<Rightarrow> list (slot := []) |
-      Some p \<Rightarrow> if (p = slot) then list(p := list_remove (list p) slot) else list (p := list_replace_list (list p) slot (list slot), slot := [])))"
+      Some p \<Rightarrow> if p = slot
+                then list(p := list_remove (list p) slot)
+                else list (p := list_replace_list (list p) slot (list slot), slot := []))"
 
 definition create_cap_ext where
 "create_cap_ext \<equiv> (\<lambda> untyped dest dest_p. do
@@ -519,86 +376,6 @@ definition work_units_limit_reached where
      return (work_units_limit \<le> work_units)
    od"
 
-text \<open>
-  A type class for all instantiations of the abstract specification. In
-  practice, this is restricted to basically allow only two sensible
-  implementations at present: the deterministic abstract specification and
-  the nondeterministic one.
-\<close>
-class state_ext =
- fixes unwrap_ext :: "'a state \<Rightarrow> det_ext state"
- fixes wrap_ext :: "(det_ext \<Rightarrow> det_ext) \<Rightarrow> ('a \<Rightarrow> 'a)"
- fixes wrap_ext_op :: "unit det_ext_monad \<Rightarrow> ('a state,unit) nondet_monad"
- fixes wrap_ext_bool :: "bool det_ext_monad \<Rightarrow> ('a state,bool) nondet_monad"
- fixes select_switch :: "'a \<Rightarrow> bool"
- fixes ext_init :: "'a"
-
-definition detype_ext :: "obj_ref set \<Rightarrow> 'z::state_ext \<Rightarrow> 'z" where
- "detype_ext S \<equiv> wrap_ext (\<lambda>s. s\<lparr>ekheap_internal := (\<lambda>x. if x \<in> S then None else ekheap_internal s x)\<rparr>)"
-
-instantiation  det_ext_ext :: (type) state_ext
-begin
-
-definition "unwrap_ext_det_ext_ext == (\<lambda>x. x) :: det_ext state \<Rightarrow> det_ext state"
-
-definition "wrap_ext_det_ext_ext == (\<lambda>x. x) ::
-  (det_ext \<Rightarrow> det_ext) \<Rightarrow> det_ext \<Rightarrow> det_ext"
-
-definition "wrap_ext_op_det_ext_ext == (\<lambda>x. x) ::
-  (det_ext state \<Rightarrow> ((unit \<times> det_ext state) set) \<times> bool)
-  \<Rightarrow> det_ext state  \<Rightarrow> ((unit \<times> det_ext state) set) \<times> bool"
-
-definition "wrap_ext_bool_det_ext_ext == (\<lambda>x. x) ::
-  (det_ext state \<Rightarrow> ((bool \<times> det_ext state) set) \<times> bool)
-  \<Rightarrow> det_ext state \<Rightarrow> ((bool \<times> det_ext state) set) \<times> bool"
-
-definition "select_switch_det_ext_ext == (\<lambda>_. True)  :: det_ext\<Rightarrow> bool"
-
-(* this probably doesn't satisfy the invariants *)
-definition "ext_init_det_ext_ext \<equiv>
-     \<lparr>work_units_completed_internal = 0,
-      scheduler_action_internal = resume_cur_thread,
-      ekheap_internal = Map.empty (idle_thread_ptr \<mapsto> default_etcb),
-      domain_list_internal = [(0,15)],
-      domain_index_internal = 0,
-      cur_domain_internal = 0,
-      domain_time_internal = 15,
-      ready_queues_internal = const (const []),
-      cdt_list_internal = const []\<rparr> :: det_ext"
-
-instance ..
-
-end
-
-section "Nondeterministic Abstract Specification"
-
-text \<open>\label{s:nondet-spec}
-The nondeterministic abstract specification instantiates the extended state
-with the unit type -- i.e. it doesn't have any meaningful extended state.
-\<close>
-
-instantiation unit :: state_ext
-begin
-
-
-definition "unwrap_ext_unit == (\<lambda>_. undefined) :: unit state \<Rightarrow> det_ext state"
-
-definition "wrap_ext_unit == (\<lambda>f s. ()) :: (det_ext \<Rightarrow> det_ext) \<Rightarrow> unit \<Rightarrow> unit"
-
-
-definition "wrap_ext_op_unit == (\<lambda>m. return ()) ::
-  (det_ext state \<Rightarrow> ((unit \<times> det_ext state) set) \<times> bool) \<Rightarrow> unit state \<Rightarrow> ((unit \<times> unit state) set) \<times> bool"
-
-definition "wrap_ext_bool_unit == (\<lambda>m. select UNIV) ::
-  (det_ext state \<Rightarrow> ((bool \<times> det_ext state ) set) \<times> bool) \<Rightarrow> unit state \<Rightarrow> ((bool \<times> unit state) set) \<times> bool"
-
-definition "select_switch_unit == (\<lambda>s. False) :: unit \<Rightarrow> bool"
-
-definition "ext_init_unit \<equiv> () :: unit"
-
-instance ..
-
-end
 
 text \<open>Run an extended operation over the extended state without
   modifying it and use the return value to choose between two computations
@@ -638,14 +415,16 @@ text \<open>
   Use the extended state to choose a value from a bounding set @{term S} when
   @{term select_switch} is true. Otherwise just select from @{term S}.
 \<close>
-definition select_ext :: "(det_ext state \<Rightarrow> 'd) \<Rightarrow> ('d set) \<Rightarrow> ('a::state_ext state,'d) nondet_monad" where
+definition select_ext ::
+  "(det_ext state \<Rightarrow> 'd) \<Rightarrow> 'd set \<Rightarrow> ('a::state_ext state,'d) nondet_monad" where
   "select_ext a S \<equiv> do
-                      s \<leftarrow> get;
-                      x \<leftarrow> if (select_switch (exst s)) then (return (a (unwrap_ext s)))
-                          else (select S);
-                      assert (x \<in> S);
-                      return x
-                    od"
+     s \<leftarrow> get;
+     x \<leftarrow> if select_switch (exst s)
+          then return (a (unwrap_ext s))
+          else select S;
+     assert (x \<in> S);
+     return x
+   od"
 
 (*Defined here because it's asserted before empty_slot*)
 definition valid_list_2 :: "cdt_list \<Rightarrow> cdt \<Rightarrow> bool" where
